extraction/theories/ErasureFunction.v
@@ -1,0 +1,567 @@
+
+From Coq Require Import Bool String List Program BinPos Compare_dec Omega.
+From MetaCoq.Template Require Import config utils monad_utils BasicAst AstUtils.
+From MetaCoq.PCUIC Require Import PCUICAst PCUICAstUtils PCUICInduction PCUICTyping PCUICChecker PCUICMetaTheory PCUICWcbvEval PCUICSafeChecker PCUICLiftSubst PCUICInversion PCUICSR PCUICNormal PCUICSafeReduce.
+From MetaCoq.Extraction Require EAst ELiftSubst ETyping EWcbvEval Extract ExtractionCorrectness.
+From Equations Require Import Equations.
+Require Import String.
+Local Open Scope string_scope.
+Set Asymmetric Patterns.
+Import MonadNotation.
+
+Existing Instance config.default_checker_flags.
+
+Definition is_prop_sort s :=
+  match Universe.level s with
+  | Some l => Level.is_prop l
+  | None => false
+  end.
+
+Require Import Extract.
+
+Fixpoint infer' Σ (HΣ : ∥wf Σ∥) (Γ : context) (HΓ : ∥ wf_local Σ Γ ∥) (t : term) {struct t}
+  : typing_result ({ A : term & ∥ Σ ;;; Γ |- t : A ∥ }).
+Admitted.
+
+Definition Is_conv_to_Arity Σ Γ T := exists T', ∥red Σ Γ T T'∥ /\ isArity T'.
+
+Ltac terror := try match goal with [t : type_error |- typing_result _] => exact (TypeError t) end.
+
+Fixpoint is_arity Σ (HΣ : wf Σ) Γ (HΓ : wf_local Σ Γ) T (HT : PCUICSafeLemmata.wellformed Σ Γ T) : typing_result ({Is_conv_to_Arity Σ Γ T} + {~ Is_conv_to_Arity Σ Γ T}).
+Proof.
+  edestruct @reduce_to_sort with (t := T) as [[u] | ]; try eassumption.
+  - left. left. sq. econstructor. split.
+    sq. eassumption. econstructor.
+  - clear t. edestruct @reduce_to_prod with (t := T); try eassumption.
+    + destruct a as (? & ? & ? & ?).
+      edestruct (is_arity Σ HΣ (Γ ,, vass x x0)) with (T := x1).
+      * enough (∥ wf_local Σ (Γ,, vass x x0) ∥) by admit. destruct HT as [ [] | []];  sq.
+        -- econstructor; cbn; eauto.
+           eapply subject_reduction in X; eauto.
+           eapply inversion_Prod in X as (? & ? & ? & ? & ?). eauto.
+        -- econstructor; cbn; eauto.
+           eapply PCUICSafeReduce.isWfArity_red in X; eauto. 
+           2: exact RedFlags.default.
+           destruct X as (? & ? & ? & ?). cbn in *.
+           admit.           
+      * sq. destruct HT as [ [] | [] ].
+        -- eapply subject_reduction in X; eauto.
+           eapply inversion_Prod in X as (? & ? & ? & ? & ?). 
+           do 2 econstructor. eauto.
+        -- econstructor 2. sq.
+           eapply PCUICSafeReduce.isWfArity_red in X; eauto. 2:exact RedFlags.default.
+           admit.           
+      * left. destruct a.
+        -- left. destruct i as (? & ? & ?). exists (tProd x x0 x2). split; sq.
+           etransitivity. eassumption. eapply PCUICReduction.red_prod. econstructor.
+           eassumption. now cbn.
+        -- right. intros (? & ? & ?). sq. 
+Admitted.      
+
+(* Fixpoint is_proposition Σ (HΣ : wf Σ) Γ (HΓ : wf_local Σ Γ) T (HT : PCUICSafeLemmata.wellformed Σ Γ T) : *)
+(*   typing_result *)
+
+Lemma arity_type_inv Σ Γ t T1 T2 :
+  Σ ;;; Γ |- t : T1 -> isArity T1 -> Σ ;;; Γ |- t : T2 -> Is_conv_to_Arity Σ Γ T2.
+Proof.
+Admitted.
+
+Lemma proposition_type_inv Σ Γ t T u :
+  Σ ;;; Γ |- t : tSort u -> is_prop_sort u -> Σ ;;; Γ |- t : T -> red Σ Γ T (tSort u).
+Proof.
+Admitted.
+
+Definition is_type_or_proof :
+  forall (Sigma : PCUICAst.global_context) (HΣ : ∥wf Sigma∥) (Gamma : context) (HΓ : ∥wf_local Sigma Gamma∥) (t : PCUICAst.term),
+    {r : typing_result bool & match r with
+                           | Checked true => Is_Type_or_Proof Sigma Gamma t 
+                           | Checked false => (Is_Type_or_Proof Sigma Gamma t -> False) × PCUICSafeLemmata.welltyped Sigma Gamma t
+                           | _ => True
+                           end}.
+Proof.
+  intros. destruct (@infer' _ HΣ Gamma HΓ t) as [ [T] | ].
+  2:{ exists (TypeError t0). eauto. }
+  edestruct is_arity with (Σ := Sigma) (Γ := Gamma)(T := T) as [[ | ] | ].
+  - admit.
+  - admit.
+  - sq. eapply PCUICValidity.validity in X as [_]; eauto.  destruct i.
+    econstructor 2. sq. eauto. destruct i. econstructor. econstructor. eauto.
+  - exists (Checked true). econstructor. split. admit. admit.
+  - destruct (@infer' _ HΣ Gamma HΓ T) as [ [K] | ].
+    + destruct @reduce_to_sort with (Σ := Sigma) ( Γ := Gamma) (t := K).
+      * admit.
+      * sq. eapply PCUICValidity.validity in X as [_]; eauto.  destruct i.
+        econstructor 2. sq. eauto. destruct i. econstructor. econstructor. eauto.
+      * destruct a. destruct (is_prop_sort x) eqn:E.
+        -- exists (Checked true). econstructor. split. admit.
+           right. exists x. admit.
+        -- exists (Checked false). split.
+           ++ admit.
+           ++ sq. econstructor. eauto.
+      * exists (TypeError t0). econstructor.
+    + exists (TypeError t0). econstructor.
+  - exists (TypeError t0). econstructor.
+Admitted.
+
+Section Erase.
+
+  Definition is_box c :=
+    match c with
+    | E.tBox => true
+    | _ => false
+    end.
+
+  Fixpoint mkAppBox c n :=
+    match n with
+    | 0 => c
+    | S n => mkAppBox (E.tApp c E.tBox) n
+    end.
+
+  Definition on_snd_map {A B C} (f : B -> C) (p : A * B) :=
+    (fst p, f (snd p)).
+
+  Variable (Σ : global_context)( HΣ :∥ wf Σ ∥).
+      
+  Ltac sq :=
+    repeat match goal with
+           | H : ∥ _ ∥ |- _ => destruct H; try clear H
+           end; try eapply sq.
+
+  Section EraseMfix.
+    Context (erase : forall  (Γ : context) (HΓ : ∥ wf_local Σ Γ ∥) (t : term), typing_result E.term).
+
+    Program Definition erase_mfix Γ (HΓ : ∥wf_local Σ Γ∥) (defs : mfixpoint term) : typing_result (EAst.mfixpoint E.term) :=
+      let Γ' := (PCUICLiftSubst.fix_context defs ++ Γ)%list in
+      monad_map (fun d => H <- _ ;;
+                   dbody' <- erase Γ' H d.(dbody);;
+                          ret ({| E.dname := d.(dname); E.rarg := d.(rarg);
+                                  E.dbody := dbody' |})) defs.
+    Next Obligation.
+      clear erase.
+      
+      epose proof ((fix check_types (mfix : mfixpoint term) acc (Hacc : ∥ wf_local_rel Σ Γ acc ∥) {struct mfix}
+              : typing_result (∥ wf_local_rel Σ (Γ ,,, acc) (fix_context_i #|acc| mfix) ∥)
+              := match mfix with
+                 | [] => ret (sq wf_local_rel_nil)
+                 | def :: mfix =>
+       (* probably not tail recursive but needed so that next line terminates *)
+                   W <- infer_type infer Γ HΓ (dtype def) ;;
+                   let W' := weakening_sq acc _ _ W.π2 in
+                   Z <- check_types mfix
+                     (acc ,, vass (dname def) ((lift0 #|acc|) (dtype def)))
+                     (wf_local_rel_abs_sq Hacc (W.π1; W')) ;;
+                   ret (wf_local_rel_app_inv_sq
+                          (wf_local_rel_abs_sq (sq wf_local_rel_nil) (W.π1; W')) Z)
+                 end)
+           defs [] (sq _)).
+      destruct X. econstructor.
+
+      
+      sq. eapply wf_local_local_rel.
+      eapply wf_local_rel_app_inv. eapply wf_local_rel_local. eauto.
+      change fix_context with (fix_context_i #|@nil context_decl|).
+      now rewrite app_context_nil_l.
+      sq. econstructor 2. exact t.
+      Unshelve. (* I believe those go away once infer works on squashed assumptions *)
+    Admitted.
+      
+  End EraseMfix.
+
+  (* Program Fixpoint erase (Γ : context) (HΓ : ∥wf_local Σ Γ∥) (t : term) {struct t} : typing_result E.term := *)
+  (*   match is_type_or_proof Σ HΣ Γ HΓ t with *)
+  (*   | (Checked true ; H) => ret (E.tBox) *)
+  (*   | (TypeError t ; H) => TypeError t *)
+  (*   | (Checked false ; H ) => (match t with *)
+  (*                             | tRel i => ret (E.tRel i) *)
+  (*                             | tVar n =>  ret (E.tVar n) *)
+  (*                             | tEvar m l => *)
+  (*                               l' <- monad_map (erase Γ HΓ) l;; *)
+  (*                                  ret (E.tEvar m l') *)
+  (*                             | tSort u =>  ret E.tBox *)
+  (*                             | tConst kn u =>  ret (E.tConst kn) *)
+  (*                             | tInd kn u =>  ret E.tBox *)
+  (*                             | tConstruct kn k u =>  ret (E.tConstruct kn k) *)
+  (*                             | tProd na b t =>  ret E.tBox *)
+  (*                             | tLambda na b t => *)
+  (*                               t' <- erase (vass na b :: Γ) _ t;; *)
+  (*                                  ret (E.tLambda na t') *)
+  (*                             | tLetIn na b t0 t1 => *)
+  (*                               b' <- erase Γ HΓ b;; *)
+  (*                                  t1' <- erase (vdef na b t0 :: Γ) _ t1;; *)
+  (*                                  ret (E.tLetIn na b' t1') *)
+  (*                             | tApp f u => *)
+  (*                               f' <- erase Γ HΓ f;; *)
+  (*                                  l' <- erase Γ HΓ u;; *)
+  (*                                  ret (E.tApp f' l') *)
+  (*                             | tCase ip p c brs => *)
+  (*                               c' <- erase Γ HΓ c;; *)
+  (*                                  brs' <- monad_map (T:=typing_result) (fun x => x' <- erase Γ HΓ (snd x);; ret (fst x, x')) brs;; *)
+  (*                                  ret (E.tCase ip c' brs') *)
+  (*                             | tProj p c => *)
+  (*                               c' <- erase Γ HΓ c;; *)
+  (*                                  ret (E.tProj p c') *)
+  (*                             | tFix mfix n => *)
+  (*                               mfix' <- erase_mfix (erase) Γ HΓ mfix;; *)
+  (*                                     ret (E.tFix mfix' n) *)
+  (*                             | tCoFix mfix n => *)
+  (*                               mfix' <- erase_mfix (erase) Γ HΓ mfix;; *)
+  (*                                     ret (E.tCoFix mfix' n) *)
+  (*                             end) *)
+  (*   end. *)
+  (* Next Obligation. *)
+  (*   destruct w. sq. econstructor; eauto. cbn. clear Heq_anonymous. *)
+        
+  (*   eapply inversion_Lambda in t0 as (? & ? & ? & ? & ?). *)
+  (*   econstructor; cbn; eauto. *)
+  (* Defined. *)
+  (* Next Obligation. *)
+  (*   destruct w. sq. econstructor; eauto. cbn. clear Heq_anonymous. *)
+  (*   eapply inversion_LetIn in t as (? & ? & ? & ? & ? & ?). *)
+  (*   econstructor; cbn; eauto. *)
+  (* Defined. *)
+
+  
+  
+  Equations(noind) erase (Γ : context) (HΓ : ∥ wf_local Σ Γ ∥) (t : term) : typing_result E.term :=
+    erase Γ HΓ t with (is_type_or_proof Σ HΣ Γ HΓ t) :=
+    {
+      erase Γ HΓ _ (Checked true ; _) := ret (E.tBox);
+      erase Γ HΓ _ (TypeError t ; _) := TypeError t ;
+      erase Γ HΓ (tRel i) _ := ret (E.tRel i) ;
+      erase Γ HΓ (tVar n) _ := ret (E.tVar n) ;
+      erase Γ HΓ (tEvar m l) _ := l' <- monad_map (erase Γ HΓ) l;; ret (E.tEvar m l') ;
+      erase Γ HΓ (tSort u) _ := ret E.tBox
+
+      ; erase Γ HΓ (tConst kn u) _ := ret (E.tConst kn)
+      ; erase Γ HΓ (tInd kn u) _ := ret E.tBox
+      ; erase Γ HΓ (tConstruct kn k u) _ := ret (E.tConstruct kn k)
+      ; erase Γ HΓ (tProd na b t) _ := ret E.tBox
+      ; erase Γ HΓ (tLambda na b t) _ :=
+                           t' <- erase (vass na b :: Γ) _ t;;
+                              ret (E.tLambda na t')
+      ; erase Γ HΓ (tLetIn na b t0 t1) _ :=
+                              b' <- erase Γ HΓ b;;
+                                 t1' <- erase (vdef na b t0 :: Γ) _ t1;;
+                                 ret (E.tLetIn na b' t1')
+      ; erase Γ HΓ (tApp f u) _ :=
+                     f' <- erase Γ HΓ f;;
+                        l' <- erase Γ HΓ u;;
+                        ret (E.tApp f' l')
+      ; erase Γ HΓ (tCase ip p c brs) _ :=
+                             c' <- erase Γ HΓ c;;
+                                brs' <- monad_map (T :=typing_result) (fun x => x' <- erase Γ HΓ (snd x);; ret (fst x, x')) brs;;
+                                ret (E.tCase ip c' brs')
+      ; erase Γ HΓ (tProj p c) _ :=
+                      c' <- erase Γ HΓ c;;
+                         ret (E.tProj p c')
+      ; erase Γ HΓ (tFix mfix n) _ :=
+                        mfix' <- erase_mfix (erase) Γ HΓ mfix;;
+                              ret (E.tFix mfix' n)
+      ; erase Γ HΓ (tCoFix mfix n) _ :=
+                          mfix' <- erase_mfix (erase) Γ HΓ mfix;;
+                                ret (E.tCoFix mfix' n)
+    }.
+  Next Obligation.
+    destruct w. sq. econstructor; eauto. cbn.
+        
+    eapply inversion_Lambda in X as (? & ? & ? & ? & ?).
+    econstructor; cbn; eauto.
+  Qed.
+  Next Obligation.
+    destruct w. sq. econstructor; eauto. cbn.
+    eapply inversion_LetIn in X as (? & ? & ? & ? & ? & ?).
+    econstructor; cbn; eauto.
+  Qed.
+  
+  (* Fixpoint erase (Γ : context) (HΓ : ∥wf_local Σ Γ∥) (t : term) {struct t} : typing_result E.term. *)
+  (* Proof. *)
+  (*   destruct (is_type_or_proof Σ HΣ Γ HΓ t) eqn:E1. *)
+  (*   destruct x as [b | ] eqn:E2. *)
+  (*   destruct b eqn:E3. *)
+  (*   - exact (ret (E.tBox)). *)
+  (*   - revert y E1. refine (match t with *)
+  (*            | tRel i => fun _ _ => ret (E.tRel i) *)
+  (*            | tVar n => fun _ _ =>  ret (E.tVar n) *)
+  (*            | tEvar m l => fun _ _ => *)
+  (*              l' <- monad_map (erase Γ HΓ) l;; *)
+  (*                 ret (E.tEvar m l') *)
+  (*            | tSort u => fun _ _ =>  ret E.tBox *)
+  (*            | tConst kn u => fun _ _ =>  ret (E.tConst kn) *)
+  (*            | tInd kn u => fun _ _ =>  ret E.tBox *)
+  (*            | tConstruct kn k u => fun _ _ =>  ret (E.tConstruct kn k) *)
+  (*            | tProd na b t => fun _ _ =>  ret E.tBox *)
+  (*            | tLambda na b t => fun _ _ => *)
+  (*              t' <- erase (vass na b :: Γ) _ t;; *)
+  (*                 ret (E.tLambda na t') *)
+  (*            | tLetIn na b t0 t1 => fun _ _ => *)
+  (*              b' <- erase Γ HΓ b;; *)
+  (*                 t1' <- erase (vdef na b t0 :: Γ) _ t1;; *)
+  (*                 ret (E.tLetIn na b' t1') *)
+  (*            | tApp f u => fun _ _ => *)
+  (*              f' <- erase Γ HΓ f;; *)
+  (*                 l' <- erase Γ HΓ u;; *)
+  (*                 ret (E.tApp f' l') *)
+  (*            | tCase ip p c brs => fun _ _ => *)
+  (*              c' <- erase Γ HΓ c;; *)
+  (*                 brs' <- monad_map (T:=typing_result) (fun x => x' <- erase Γ HΓ (snd x);; ret (fst x, x')) brs;; *)
+  (*                 ret (E.tCase ip c' brs') *)
+  (*            | tProj p c => fun _ _ => *)
+  (*              c' <- erase Γ HΓ c;; *)
+  (*                 ret (E.tProj p c') *)
+  (*            | tFix mfix n => fun _ _ => *)
+  (*                mfix' <- erase_mfix (erase) Γ HΓ mfix;; *)
+  (*                ret (E.tFix mfix' n) *)
+  (*            | tCoFix mfix n => fun _ _ => *)
+  (*                mfix' <- erase_mfix (erase) Γ HΓ mfix;; *)
+  (*                ret (E.tCoFix mfix' n) *)
+  (*             end). *)
+      
+  (*     + destruct p as [? []]. sq. clear e. *)
+        
+  (*       eapply inversion_Lambda in t1 as (? & ? & ? & ? & ?). *)
+  (*       econstructor; cbn; eauto. *)
+  (*     + destruct p as [? []]. sq. clear e. *)
+                
+  (*       eapply inversion_LetIn in t2 as (? & ? & ? & ? & ? & ?). *)
+  (*       econstructor; cbn; eauto. *)
+  (*   - exact (TypeError t0). *)
+  (* Defined. *)
+
+End Erase.
+
+Require Import ExtractionCorrectness.
+
+Lemma erases_erase Σ Γ t T (wfΣ : ∥wf Σ∥) (wfΓ : ∥wf_local Σ Γ∥) t' :
+  Σ ;;; Γ |- t : T ->
+  erase Σ (wfΣ) Γ (wfΓ) t = Checked t' ->                
+  erases Σ Γ t t'.
+Proof.
+  Hint Constructors typing erases.
+  intros. sq.
+  (* pose proof (typing_wf_local X0). *)
+
+    
+  pose (wfΣ' := sq t0).
+  pose (wfΓ' := sq a).
+  change (erase Σ wfΣ' Γ wfΓ' t = Checked t') in H.
+
+  revert H.
+  generalize wfΣ' wfΓ'. clear wfΣ' wfΓ'.
+  
+  revert Σ t0 Γ a t T X t'.
+  eapply (typing_ind_env (fun Σ Γ t T =>   forall (t' : E.term) (wfΣ' : ∥ wf Σ ∥) (wfΓ' : ∥ wf_local Σ Γ ∥),
+  erase Σ wfΣ' Γ wfΓ' t = Checked t' -> Σ;;; Γ |- t ⇝ℇ t'
+         )); intros.
+
+  all:eauto.
+  all: simp erase in *.
+  all: unfold erase_clause_1 in *.
+
+  all: cbn in *; repeat (destruct ?;  repeat match goal with
+                                          [ H : Checked _ = Checked _ |- _ ] => inv H
+                                        | [ H : TypeError _ = Checked _ |- _ ] => inv H
+                                        | [ H : _ × PCUICSafeLemmata.welltyped _ _ _ |- _ ] => destruct H as [? []]
+                                        end; eauto).
+    
+  - repeat econstructor; eauto.
+  - econstructor. econstructor. clear E.
+    eapply inversion_Prod in t0 as (? & ? & ? & ? & ?).
+    split. eauto. left. econstructor.
+  - econstructor. eauto. econstructor. clear E.
+    eapply inversion_Ind in t as (? & ? & ? & ? & ? & ?).
+    split. eauto. left.
+    eapply isArity_subst_instance. eapply isArity_ind_type.
+  - econstructor.
+    eapply elim_restriction_works. intros.
+    eapply f, Is_Type_or_Proof_Proof. eauto. eauto.
+    
+    pose proof (Prelim.monad_map_All2 _ _ _ brs a1 E3).
+    
+    eapply All2_All_left in X3. 2:{ intros. destruct X4. exact e. }
+
+    eapply All2_impl.
+    eapply All2_All_mix_left. eassumption. eassumption.
+    intros. destruct H5.
+    destruct ?; inv e0. cbn. eauto.
+  - econstructor.
+
+    eapply elim_restriction_works_proj. intros.
+    eapply Is_Type_or_Proof_Proof in X2. eauto.
+
+    eauto.
+  - econstructor.
+    unfold erase_mfix in *.
+    pose proof (Prelim.monad_map_All2 _ _ _ mfix a0 E2).
+    eapply All2_impl. eapply All2_All_mix_left. eassumption. eassumption.
+
+    intros. destruct X1. cbn in *. repeat destruct ?; inv e. 
+    cbn. repeat split; eauto. 
+    eapply p. eauto. 
+  - econstructor.
+    unfold erase_mfix in *.
+    pose proof (Prelim.monad_map_All2 _ _ _ mfix a0 E2).
+    eapply All2_impl. eapply All2_All_mix_left. eassumption. eassumption.
+
+    intros. destruct X1. cbn in *. repeat destruct ?; inv e.
+    cbn. repeat split; eauto. 
+    eapply p. eauto.
+Qed.
+
+Definition optM {M : Type -> Type} `{Monad M} {A B} (x : option A) (f : A -> M B) : M (option B) :=
+  match x with
+  | Some x => y <- f x ;; ret (Some y)
+  | None => ret None
+  end.
+
+Lemma wf_local_nil {Σ} : ∥ wf_local Σ [] ∥.
+Proof. repeat econstructor. Qed.
+
+Definition erase_constant_body Σ wfΣ (cb : constant_body) : typing_result E.constant_body :=
+  ty <- erase Σ wfΣ [] wf_local_nil cb.(cst_type) ;;
+  body <- optM cb.(cst_body) (fun b => erase Σ wfΣ [] wf_local_nil b);;
+  ret {| E.cst_body := body; |}.
+
+Definition lift_opt_typing {A} (a : option A) (e : type_error) : typing_result A :=
+  match a with
+  | Some x => ret x
+  | None => raise e
+  end.
+
+Definition erase_one_inductive_body Σ wfΣ npars arities Har
+           (oib : one_inductive_body) : typing_result E.one_inductive_body :=
+  decty <- lift_opt_typing (decompose_prod_n_assum [] npars oib.(ind_type))
+        (NotAnInductive oib.(ind_type)) ;;
+  let '(params, arity) := decty in
+  type <- erase Σ wfΣ [] wf_local_nil oib.(ind_type) ;;
+  ctors <- monad_map (fun '(x, y, z) => y' <- erase Σ wfΣ arities Har y;; ret (x, y', z)) oib.(ind_ctors);;
+  let projctx := arities ,,, params ,, vass nAnon oib.(ind_type) in
+  projs <- monad_map (fun '(x, y) => y' <- erase Σ wfΣ [] wf_local_nil y;; ret (x, y')) oib.(ind_projs);;
+  ret {| E.ind_name := oib.(ind_name);
+         E.ind_kelim := oib.(ind_kelim);
+         E.ind_ctors := ctors;
+         E.ind_projs := projs |}.
+
+Program Definition erase_mutual_inductive_body Σ wfΣ
+           (mib : mutual_inductive_body) (Hm :   ∥ wf_local Σ (arities_context (ind_bodies mib)) ∥)
+: typing_result E.mutual_inductive_body :=
+  let bds := mib.(ind_bodies) in
+  let arities := arities_context bds in
+  bodies <- monad_map (erase_one_inductive_body Σ wfΣ mib.(ind_npars) arities _) bds ;;
+  ret {| E.ind_npars := mib.(ind_npars);
+         E.ind_bodies := bodies; |}.
+
+Program Fixpoint erase_global_decls univs Σ : ∥ wf (Σ, univs) ∥ -> typing_result E.global_declarations := fun wfΣ =>
+  match Σ with
+  | [] => ret []
+  | ConstantDecl kn cb :: Σ => 
+    cb' <- erase_constant_body (Σ, univs) _ cb;;
+    Σ' <- erase_global_decls univs Σ _;;
+    ret (E.ConstantDecl kn cb' :: Σ')
+  | InductiveDecl kn mib :: Σ => 
+    mib' <- erase_mutual_inductive_body (Σ, univs) _ mib _ ;;
+    Σ' <- erase_global_decls univs Σ _;;
+    ret (E.InductiveDecl kn mib' :: Σ')
+  end.
+Next Obligation.
+  sq. eapply PCUICWeakeningEnv.wf_extends. eauto. eexists [_]; reflexivity.
+Qed.
+Next Obligation.
+  sq. eapply PCUICWeakeningEnv.wf_extends. eauto. eexists [_]; reflexivity.
+Qed.
+Next Obligation.
+  Require Import MetaCoq.PCUIC.PCUICWeakeningEnv.
+  sq. eapply wf_extends; eauto. eexists [_]; reflexivity.
+Qed.
+Next Obligation.
+  sq. inv X. cbn in *.
+  eapply PCUICSubstitution.wf_arities_context'; eauto.
+Qed.
+Next Obligation.
+  sq. eapply PCUICWeakeningEnv.wf_extends. eauto. eexists [_]; reflexivity.
+Qed.
+
+Program Definition erase_global Σ : ∥wf Σ∥ -> _:=
+  match Σ with (Σ, univs) => fun wfΣ  =>
+  Σ' <- erase_global_decls univs Σ wfΣ ;;
+  ret Σ' end.
+
+           
+Lemma constructors_typed:
+  forall (Σ : list global_decl) (univs : constraints) (k : kername)
+    (m : mutual_inductive_body) (x : one_inductive_body) (t1 : term) 
+    (i0 : ident) (n0 : nat),
+    In (i0, t1, n0) (ind_ctors x) ->
+    on_inductive (fun Σ0 : global_context => lift_typing typing Σ0) (Σ, univs) k m ->
+    ∑ T, (Σ, univs);;; arities_context (ind_bodies m) |- t1 : T.
+Proof.
+  intros Σ univs k m x t1 i0 n0 H2 X0.
+Admitted.
+
+Lemma proj_typed:
+  forall (Σ : list global_decl) (univs : constraints) (k : kername)
+    (m : mutual_inductive_body) (x : one_inductive_body) (t1 : term) 
+    (i0 : ident) (H2 : In (i0, t1) (ind_projs x))
+    (X0 : on_inductive (fun Σ0 : global_context => lift_typing typing Σ0) (Σ, univs) k m),
+    ∑ T, (Σ, univs);;; [] |- t1 : T.
+Proof.
+  
+Admitted.
+
+Lemma erase_global_correct Σ (wfΣ : ∥ wf Σ∥) Σ' :
+  erase_global Σ wfΣ = Checked Σ' ->
+  erases_global Σ Σ'.
+Proof.
+  destruct Σ as (Σ, univs).
+  induction Σ in wfΣ, Σ' |- *; cbn; intros; sq.
+  - inv H. econstructor.
+  - repeat destruct ?; try congruence.
+    + inv H. inv E. inv E1. econstructor.
+      * unfold erases_constant_body.
+        unfold optM in E4. destruct ?; try congruence.
+        -- cbn. cbn in *.
+           destruct ( erase (Σ, univs)
+           (erase_global_decls_obligation_1 univs (ConstantDecl k c :: Σ) 
+              (sq t) k c Σ eq_refl) [] wf_local_nil t0) eqn:E5;
+             rewrite E5 in E4; inv E4.
+           eapply erases_erase. 2:eauto.
+           instantiate (1 := cst_type c).
+           clear - t E. inv t.
+           cbn in *. unfold on_constant_decl in X0.
+           rewrite E in X0. cbn in X0. eassumption.           
+        -- cbn. inv E4. econstructor.
+      * eapply IHΣ. unfold erase_global. rewrite E2. reflexivity.
+    + inv H. inv E. inv E1.
+      econstructor.
+      * econstructor; cbn; eauto.
+        pose proof (Prelim.monad_map_All2 _ _ _ _ _ E3).
+        eapply All2_Forall.
+        eapply All2_impl. eassumption.
+
+        intros. cbn in H0. repeat destruct ?; try congruence.
+        inv H0. unfold erases_one_inductive_body. cbn.
+        unfold lift_opt_typing in E.
+        destruct decompose_prod_n_assum eqn:E6; inv E. cbn.
+        pose proof (Prelim.monad_map_All2 _ _ _ _ _ E4). 
+        pose proof (Prelim.monad_map_All2 _ _ _ _ _ E5). repeat split; eauto.
+        -- eapply All2_Forall.
+           eapply All2_impl_In. eassumption.
+           intros. destruct x0, p, y, p. cbn in *.
+           destruct ?; try congruence.
+           inv H4. split; eauto.
+
+           pose (t' := t). inv t'. cbn in *.
+           edestruct constructors_typed; eauto.
+           eapply erases_erase. 2:eauto. eauto.
+        -- eapply All2_Forall.
+           eapply All2_impl_In. eassumption.
+           intros. cbn in H2. destruct x0, y.
+           destruct ?; try congruence;
+             inv H4. split; eauto.
+
+           pose (t' := t). inv t'. cbn in *.
+           edestruct proj_typed; eauto.
+           
+           eapply erases_erase.
+           2:{ eauto. } eauto.
+  * eapply IHΣ. unfold erase_global. rewrite E2. reflexivity.
+Qed.
