extraction/theories/ExtractionCorrectness.v
@@ -1,0 +1,1091 @@
+(* Distributed under the terms of the MIT license.   *)
+
+From Coq Require Import Bool String List Program BinPos Compare_dec Omega.
+From MetaCoq.Template Require Import config utils monad_utils BasicAst AstUtils.
+From MetaCoq.Extraction Require Import EAst ELiftSubst ETyping EWcbvEval Extract Prelim ESubstitution EInversion.
+From MetaCoq.PCUIC Require Import PCUICTyping PCUICAst PCUICAstUtils PCUICInduction  PCUICWeakening PCUICSubstitution PCUICChecker PCUICRetyping PCUICMetaTheory PCUICWcbvEval PCUICSR  PCUICClosed PCUICInversion.
+
+
+Require Import String.
+Local Open Scope string_scope.
+Set Asymmetric Patterns.
+Import MonadNotation.
+
+Module E := EAst.
+
+Require Import Lia.
+
+Existing Instance config.default_checker_flags.
+Module PA := PCUICAst.
+Module P := PCUICWcbvEval.
+
+Ltac inv H := inversion H; subst; clear H.
+
+(** ** Prelim stuff, should move *)
+
+Lemma All2_right_triv {A B} {l : list A} {l' : list B} P :
+  All P l' -> #|l| = #|l'| -> All2 (fun _ b => P b) l l'.
+Proof.
+  induction 1 in l |- *; cbn; intros; destruct l; cbn in *; try omega; econstructor; eauto.
+Qed.
+
+Lemma All_repeat {A} {n P} x :
+  P x -> @All A P (repeat x n).
+Proof.
+  induction n; cbn; econstructor; eauto.
+Qed.
+
+Lemma Alli_impl {A} {P Q} (l : list A) {n} : Alli P n l -> (forall n x, P n x -> Q n x) -> Alli Q n l.
+Proof. induction 1; try constructor; intuition auto. Defined.
+
+
+Lemma All2_map_left {A B C} (P : A -> C -> Type) l l' (f : B -> A) :
+  All2 (fun x y => P (f x) y) l l' -> All2 P  (map f l) l'.
+Proof. intros. rewrite <- (map_id l'). eapply All2_map; eauto. Qed.
+
+Lemma All2_map_right {A B C} (P : A -> C -> Type) l l' (f : B -> C) :
+  All2 (fun x y => P x (f y)) l l' -> All2 P  l (map f l').
+Proof. intros. rewrite <- (map_id l). eapply All2_map; eauto. Qed.
+
+Lemma Forall2_Forall_right {A B} {P : A -> B -> Prop} {Q : B -> Prop} {l l'} :
+  Forall2 P l l' ->
+  (forall x y, P x y -> Q y) ->
+  Forall Q l'.
+Proof.
+  intros HF H. induction HF; constructor; eauto.
+Qed.
+
+Lemma All2_from_nth_error A B L1 L2 (P : A -> B -> Type) :
+  #|L1| = #|L2| ->
+                (forall n x1 x2, n < #|L1| -> nth_error L1 n = Some x1
+                                      -> nth_error L2 n = Some x2
+                                      -> P x1 x2) ->
+                All2 P L1 L2.
+Proof.
+  revert L2; induction L1; cbn; intros.
+  - destruct L2; inv H. econstructor.
+  - destruct L2; inv H. econstructor.
+    eapply (X 0); cbn; eauto. omega.
+    eapply IHL1. eauto.
+    intros. eapply (X (S n)); cbn; eauto. omega.
+Qed.
+
+Lemma All2_nth_error {A B} {P : A -> B -> Type} {l l'} n t t' :
+  All2 P l l' ->
+  nth_error l n = Some t ->
+  nth_error l' n = Some t' ->
+  P t t'.
+Proof.
+  intros Hall. revert n.
+  induction Hall; destruct n; simpl; try congruence.
+  eauto.
+Qed.
+
+Lemma All_In X (P : X -> Type) (l : list X) x : All P l -> In x l -> squash (P x).
+Proof.
+  induction 1; cbn; intros; destruct H.
+  - subst. econstructor. eauto.
+  - eauto.
+Qed.      
+
+Lemma nth_error_skipn A l m n (a : A) :
+  nth_error l (m + n) = Some a ->
+  nth_error (skipn m l) n = Some a.
+Proof.
+  induction m in n, l |- *.
+  - cbn. destruct l; firstorder.
+  - cbn. destruct l.
+    + inversion 1.
+    + eapply IHm.
+Qed.
+
+Lemma declared_inductive_inj {Σ mdecl mdecl' ind idecl idecl'} :
+  declared_inductive Σ mdecl' ind idecl' ->
+  declared_inductive Σ mdecl ind idecl ->
+  mdecl = mdecl' /\ idecl = idecl'.
+Proof.
+  intros [] []. unfold declared_minductive in *.
+  rewrite H in H1. inv H1. rewrite H2 in H0. inv H0. eauto.
+Qed.
+
+Lemma decompose_app_rec_inv2 {t l' f l} :
+  decompose_app_rec t l' = (f, l) ->
+  isApp f = false.
+Proof.
+  induction t in f, l', l |- *; try intros [= <- <-]; try reflexivity.
+  simpl. apply IHt1.
+Qed.
+
+Module Ee := EWcbvEval.
+
+Lemma value_app_inv L :
+  Ee.value (E.mkApps tBox L) ->
+  L = nil.
+Proof.
+  intros. depelim H.
+  - destruct L using rev_ind.
+    reflexivity.
+    rewrite emkApps_snoc in H. inv H.
+  - induction L using rev_ind.
+    + reflexivity.
+    + rewrite emkApps_snoc in x. inv x.
+  - induction L using rev_ind.
+    + reflexivity.
+    + rewrite emkApps_snoc in x. inv x.
+  - assert (EAst.isApp (EAst.tConstruct i k) = false) by reflexivity.
+    assert (EAst.isApp tBox = false) by reflexivity.
+    eapply Prelim.decompose_app_mkApps in H0.
+    eapply Prelim.decompose_app_mkApps in H1.
+    rewrite <- x in H1. rewrite H0 in H1.
+    inv H1.
+Qed.
+
+(** ** Prelim on eliminations  *)
+
+Lemma elim_restriction_works Σ Γ ind npar p c brs :
+  (Is_proof Σ Γ (tCase (ind, npar) p c brs) -> False) -> Informative Σ ind.
+Proof.
+Admitted.
+
+Lemma elim_restriction_works_proj Σ Γ  p c :
+  (Is_proof Σ Γ (tProj p c) -> False) -> Informative Σ (fst (fst p)).
+Proof.
+Admitted.
+
+Lemma length_of_btys {ind mdecl' idecl' args' u' p pty indctx pctx ps btys} :
+  types_of_case ind mdecl' idecl' (firstn (ind_npars mdecl') args') u' p pty = Some (indctx, pctx, ps, btys) ->
+  #|btys| = #|ind_ctors idecl'|.
+Proof.
+Admitted.
+
+Lemma tCase_length_branch_inv Σ Γ ind npar p n u args brs T m t :
+  wf Σ ->
+  Σ ;;; Γ |- tCase (ind, npar) p (mkApps (tConstruct ind n u) args) brs : T ->
+  nth_error brs n = Some (m, t) ->
+  #|args| = npar + m.
+Admitted.
+
+(** ** Prelim on fixpoints *)
+
+Lemma fix_subst_nth mfix n :
+  n < #|mfix| ->
+  nth_error (fix_subst mfix) n = Some (tFix mfix (#|mfix| - n - 1)).
+Proof.
+  unfold fix_subst. generalize (#|mfix|).
+  intros m. revert n. induction m; cbn; intros.
+  - destruct n; inv H.
+  - destruct n.
+    + cbn. now rewrite <- minus_n_O.
+    + cbn. rewrite IHm. reflexivity. omega.
+Qed.
+
+Lemma efix_subst_nth mfix n :
+  n < #|mfix| ->
+  nth_error (ETyping.fix_subst mfix) n = Some (E.tFix mfix (#|mfix| - n - 1)).
+Proof.
+  unfold ETyping.fix_subst. generalize (#|mfix|).
+  intros m. revert n. induction m; cbn; intros.
+  - destruct n; inv H.
+  - destruct n.
+    + cbn. now rewrite <- minus_n_O.
+    + cbn. rewrite IHm. reflexivity. omega.
+Qed.
+
+Lemma subslet_fix_subst Σ mfix1 :
+  subslet Σ [] (PCUICTyping.fix_subst mfix1) (PCUICLiftSubst.fix_context mfix1).
+Proof.
+Admitted.
+
+(** ** Prelim on typing *)
+
+Lemma typing_subst_instance Σ Γ t T u :
+  wf Σ ->
+  Σ ;;; Γ |- t : T ->
+  Σ ;;; Γ |- PCUICUnivSubst.subst_instance_constr u t : PCUICUnivSubst.subst_instance_constr u T.
+Proof.
+Admitted.
+
+Require Import PCUIC.PCUICGeneration.
+
+Inductive red_decls Σ Γ Γ' : forall (x y : PCUICAst.context_decl), Type :=
+| conv_vass na na' T T' : isWfArity_or_Type Σ Γ' T' -> red Σ Γ T T' ->
+                      red_decls Σ Γ Γ' (PCUICAst.vass na T) (PCUICAst.vass na' T')
+
+| conv_vdef_type na na' b T T' : isWfArity_or_Type Σ Γ' T' -> red Σ Γ T T' ->
+                             red_decls Σ Γ Γ' (PCUICAst.vdef na b T) (PCUICAst.vdef na' b T')
+
+| conv_vdef_body na na' b b' T : Σ ;;; Γ' |- b' : T -> red Σ Γ b b' ->
+                                                  red_decls Σ Γ Γ' (PCUICAst.vdef na b T) (PCUICAst.vdef na' b' T).
+
+Notation red_context := (context_relation red_decls).
+
+Lemma env_prop_imp `{checker_flags} P1 P2 :
+  (forall Σ Γ t T, P1 Σ Γ t T -> P2 Σ Γ t T) ->
+  env_prop P1 -> env_prop P2.
+Proof.
+  (* intros. econstructor; *)
+  (*           specialize (X0 Σ wfΣ Γ wfΓ t T). *)
+  (* 2: now eapply X, X0. *)
+  (* destruct X0; eauto. cbv. destruct Σ. cbv in f. *)
+  (* clear - X f. *)
+  (* induction f. *)
+  (* - econstructor. eauto. *)
+  (* - econstructor. eapply IHf; eauto. *)
+  (*   eauto. destruct d. cbn in *. *)
+  (*   + destruct c0. cbv in *. *)
+  (*     destruct cst_body. eapply X. eauto. *)
+  (*     destruct o as []. exists x. *)
+  (*     eauto. *)
+  (*   + clear IHf. cbv in *. *)
+  (*     inv o. econstructor; eauto. *)
+  (*     * eapply Alli_impl. eassumption. intros.  *)
+  (*       inv X0. *)
+  (*       unshelve epose (_ : (on_constructors *)
+  (*                              (fun (Σ : list PCUICAst.global_decl × Universes.ConstraintSet.t_) (Γ : list PCUICAst.context_decl)  *)
+  (*                                 (t : PCUICAst.term) (T : option PCUICAst.term) => *)
+  (*                                 match T with *)
+  (*                                 | Some T0 => P2 Σ Γ t T0 *)
+  (*                                 | None => ∑ s : ∑ l : list (Universes.Level.t × bool), [] = l -> False, P2 Σ Γ t (PCUICAst.tSort s) *)
+  (*                                 end) (Σ, c) k m n x (PCUICAst.ind_ctors x)) *)
+  (*                      ). *)
+  (*       { *)
+  (*         clear - onConstructors X. eapply Alli_impl. eassumption. *)
+  (*         intros. inv X0. econstructor. inv X1. exists x1. eauto. *)
+  (*         destruct X2. exists x1. admit. *)
+  (*       }  *)
+        
+  (*       econstructor. eassumption. inv onArity. *)
+  (*       econstructor. eauto. intros. eapply onProjections in H. inv H. *)
+  (*       econstructor. all:eauto. *)
+  (*       eapply Alli_impl. eauto. intros. cbn in *. destruct X0. exists x1. eauto. *)
+  (*       instantiate (1 := o). *)
+  (*       unfold check_ind_sorts in *. *)
+  (*       destruct ?. intros. subst. destruct onConstructors. cbn in *. eauto. subst o. *)
+  (*       cbn. admit. admit. admit. *)
+  (*     * inv onParams. *)
+  (*       -- econstructor. *)
+  (*       -- econstructor. 2:{ destruct X1. eexists; eauto. } *)
+  (*          clear - X X0. induction X0. econstructor. *)
+  (*          econstructor. eauto. destruct t0. eexists; eauto. *)
+  (*          econstructor. eauto. eauto. *)
+  (*       -- unfold on_context. econstructor. *)
+  (*          2:{ eauto. } clear - X X0. induction X0. econstructor. *)
+  (*          econstructor. eauto. destruct t0. eexists; eauto. *)
+  (*          econstructor; eauto. *)
+Admitted.
+
+Lemma red_context_conversion :
+  env_prop
+    (fun (Σ : PCUICAst.global_context) (Γ : PCUICAst.context) (t T : PCUICAst.term) =>
+       forall Γ' : PCUICAst.context, red_context Σ Γ Γ' -> Σ;;; Γ' |- t : T).
+Proof.
+  eapply env_prop_imp. 2: eapply context_conversion.
+  intros. eapply X.
+  clear - X0.
+  Lemma red_conv_context:
+    forall (Σ : global_context) (Γ Γ' : context), red_context Σ Γ Γ' -> conv_context Σ Γ Γ'.
+  Proof.
+    intros Σ Γ Γ' X0.
+    induction X0.
+    - econstructor.
+    - econstructor. eauto. econstructor. inv p. eauto.
+      inv p. econstructor. now eapply PCUICCumulativity.red_cumul.
+      now eapply PCUICCumulativity.red_cumul_inv.
+    - econstructor. eauto. inv p.
+      econstructor. eauto. econstructor.
+      now eapply PCUICCumulativity.red_cumul.
+      now eapply PCUICCumulativity.red_cumul_inv.
+      econstructor. eauto.
+      econstructor.
+      now eapply PCUICCumulativity.red_cumul.
+      now eapply PCUICCumulativity.red_cumul_inv.
+  Qed.
+  now eapply red_conv_context.
+Qed.
+
+Lemma conv_context_app (Σ : global_context) (Γ1 Γ2 Γ1' Γ2' : context) :
+  conv_context Σ Γ1 Γ1' -> conv_context Σ Γ2 Γ2' -> conv_context Σ (Γ1 ,,, Γ2) (Γ1' ,,, Γ2').
+Proof.
+  intros. induction X0; cbn; eauto.
+  - econstructor. eauto. inv p. econstructor. admit. admit.
+  - econstructor. eauto. inv p. econstructor. admit. admit.
+    econstructor. admit. admit.
+Admitted.
+
+(** ** Prelim on arities and proofs *)
+
+Lemma isArity_subst_instance u T :
+  isArity T ->
+  isArity (PCUICUnivSubst.subst_instance_constr u T).
+Proof.
+  induction T; cbn; intros; tauto.
+Qed.
+
+
+Lemma isArity_ind_type:
+  forall idecl : one_inductive_body, isArity (ind_type idecl).
+Proof.
+  intros idecl.
+Admitted.
+
+
+Lemma Is_type_or_proof_instance_constr Σ Γ T u :
+  wf Σ ->  wf_local Σ Γ ->
+  Is_Type_or_Proof Σ Γ T ->
+  Is_Type_or_Proof Σ Γ (PCUICUnivSubst.subst_instance_constr u T).
+Proof.
+Admitted.
+
+Lemma Is_type_app Σ Γ t L T :
+  wf Σ ->
+  Σ ;;; Γ |- mkApps t L : T ->
+  Is_Type_or_Proof Σ Γ t ->
+  Is_Type_or_Proof Σ Γ (mkApps t L).
+Proof.
+  (* intros. eapply type_mkApps_inv in X0 as (? & ? & [] & ?); try eassumption. *)
+  (* destruct X1 as (? & ? & [ | [u]]). *)
+  (* -  *)
+
+  (*   Lemma typing_spine_change : *)
+  (*     forall (Σ : global_context) (Γ : context) (t : term) (L : list term) (x1 : term), *)
+  (*       Σ;;; Γ |- t : x1 -> forall x x0 : term, Σ;;; Γ |- t : x -> typing_spine Σ Γ x L x0 -> typing_spine Σ Γ x1 L x0. *)
+  (*   Proof. *)
+  (*     intros Σ Γ t L x1 t2 x x0 t0 t1. *)
+  (*   Admitted. *)
+  (*   eapply typing_spine_change in t1. 3:eapply t0. 2:eapply t2. clear t0. *)
+  (*   revert t t2. *)
+  (*   dependent induction t1; intros. *)
+  (*   + cbn. exists ty. split; eauto. *)
+  (*   + cbn. eapply IHt1. admit. *)
+  (*     eauto. eauto. *)
+  (* - destruct p.  *)
+Admitted.
+
+Notation "Σ ;;; Γ |- s ▷ t" := (eval Σ Γ s t) (at level 50, Γ, s, t at next level) : type_scope.
+Notation "Σ ⊢ s ▷ t" := (Ee.eval Σ s t) (at level 50, s, t at next level) : type_scope.
+
+Lemma Is_type_red Σ Γ t v:
+  wf Σ ->
+  red Σ Γ t v ->
+  Is_Type_or_Proof Σ Γ t ->
+  Is_Type_or_Proof Σ Γ v.
+Proof.
+  intros ? ? (T & ? & ?).
+  exists T. split.
+  - eapply subject_reduction; eauto.
+  - eauto.
+Qed.
+
+Lemma Is_type_eval Σ Γ t v:
+  wf Σ ->
+  eval Σ Γ t v ->
+  Is_Type_or_Proof Σ Γ t ->
+  Is_Type_or_Proof Σ Γ v.
+Proof.
+  intros; eapply Is_type_red. eauto.
+  eapply wcbeval_red; eauto. eauto.
+Qed.
+
+Lemma Is_type_lambda Σ Γ na T1 t :
+  wf Σ ->
+  Is_Type_or_Proof Σ Γ (tLambda na T1 t) ->
+  Is_Type_or_Proof Σ (vass na T1 :: Γ) t.
+Proof.
+  intros ? (T & ? & ?).
+  eapply inversion_Lambda in t0 as (? & ? & ? & ? & ?).
+  exists x0. split; eauto. destruct s as [ | (u & ? & ?)].
+  - left. admit.
+  - right. exists u. split; eauto.
+Admitted.
+
+Lemma tConstruct_no_Type Σ ind c u x1 :
+  Is_Type_or_Proof Σ [] (mkApps (tConstruct ind c u) x1) ->
+  Is_proof Σ [] (mkApps (tConstruct ind c u) x1).
+Admitted.
+
+(** * Correctness of erasure  *)
+
+Notation "Σ ;;; Γ |- s ▷ t" := (eval Σ Γ s t) (at level 50, Γ, s, t at next level) : type_scope.
+Notation "Σ ⊢ s ▷ t" := (Ee.eval Σ s t) (at level 50, s, t at next level) : type_scope.
+
+(** ** Erasure is stable under context conversion *)
+
+Lemma Is_type_conv_context  (Σ : global_context) (Γ : context) t (Γ' : context) :
+  wf Σ -> wf_local Σ Γ ->
+    conv_context Σ Γ Γ' -> Is_Type_or_Proof Σ Γ t -> Is_Type_or_Proof Σ Γ' t.
+Proof.
+  intros.
+  destruct X2 as (? & ? & ?).
+  exists x. split. eapply context_conversion; eauto.
+  destruct s as [? | [u []]].
+  - eauto.
+  - right. exists u. split; eauto. eapply context_conversion; eauto.
+Qed.
+
+Lemma erases_context_conversion :
+env_prop
+  (fun (Σ : PCUICAst.global_context) (Γ : PCUICAst.context) (t T : PCUICAst.term) =>
+      forall Γ' : PCUICAst.context, conv_context Σ Γ Γ' -> forall t', erases Σ Γ t t' -> erases Σ Γ' t t').
+Proof.
+  apply typing_ind_env; intros Σ wfΣ Γ wfΓ; intros **; rename_all_hyps.
+  all: match goal with [ H : erases _ _ ?a _ |- ?G ] => tryif is_var a then idtac else inv H end.
+  Hint Resolve Is_type_or_proof_instance_constr.
+  Hint Resolve Is_type_conv_context.
+  all: try now (econstructor; eauto).
+  - econstructor. eapply h_forall_Γ'0.
+    econstructor. eauto. econstructor. admit. econstructor; eapply cumul_refl'.
+    eassumption.
+  - econstructor. eauto. eapply h_forall_Γ'1.
+    econstructor. eauto. econstructor. admit. econstructor; eapply cumul_refl'.
+    eassumption.
+  - econstructor. eauto. eauto.
+    eapply All2_All_left in X3. 2:{ intros. destruct X1. exact e. }
+
+    eapply All2_impl. eapply All2_All_mix_left.
+    all: firstorder.
+  - econstructor.
+
+    eapply All2_impl. eapply All2_All_mix_left. eassumption. eassumption.
+    intros. cbn in *.
+    decompose [prod] X2. repeat split; eauto.
+    eapply b0. 2:eauto. subst types.
+    
+    eapply conv_context_app. eauto. eapply conv_context_refl. eauto. admit. (* wf_local fix_context *)
+  - econstructor.
+
+    eapply All2_impl. eapply All2_All_mix_left. eassumption. eassumption.
+    intros. cbn in *.
+    decompose [prod] X2. repeat split; eauto.
+    eapply b0. 2:eauto. subst types.
+  
+    eapply conv_context_app. eauto. eapply conv_context_refl. eauto. admit. (* wf_local fix_context *)
+  - eauto.
+Admitted.
+
+Lemma erases_red_context_conversion :
+env_prop
+  (fun (Σ : PCUICAst.global_context) (Γ : PCUICAst.context) (t T : PCUICAst.term) =>
+      forall Γ' : PCUICAst.context, red_context Σ Γ Γ' -> forall t', erases Σ Γ t t' -> erases Σ Γ' t t').
+Proof.
+  eapply env_prop_imp.
+  2: eapply erases_context_conversion.
+  intros. cbn in *. eapply H; eauto.
+  eapply red_conv_context; eauto.
+Qed.
+
+(** ** Erasure is stable under substituting universe constraints  *)
+
+Lemma erases_subst_instance_constr :
+  forall Σ, wf Σ ->
+  forall Γ, wf_local Σ Γ ->
+  forall t T, Σ ;;; Γ |- t : T ->
+  forall t' u,
+    Σ ;;; Γ |- t ⇝ℇ t' ->
+    Σ ;;; Γ |- PCUICUnivSubst.subst_instance_constr u t ⇝ℇ t'.
+Proof.
+  apply (typing_ind_env (fun Σ Γ t T =>
+                           forall t' u,
+                             Σ ;;; Γ |- t ⇝ℇ t' ->
+                                       Σ ;;; Γ |- PCUICUnivSubst.subst_instance_constr u t ⇝ℇ t'
+        )); intros; cbn -[PCUICUnivSubst.subst_instance_constr] in *.
+  all: match goal with [ H : erases _ _ ?a _ |- ?G ] => tryif is_var a then idtac else inv H end.
+  Hint Resolve Is_type_or_proof_instance_constr. 
+  all: try now (econstructor; eauto).
+  all:cbn.
+Admitted.
+
+(** ** Erasure and applications  *)
+
+Lemma erases_App Σ Γ f L T t :
+  Σ ;;; Γ |- tApp f L : T ->
+  erases Σ Γ (tApp f L) t ->
+  (t = tBox × squash (Is_Type_or_Proof Σ Γ (tApp f L)))
+  \/ exists f' L', t = E.tApp f' L' /\
+             erases Σ Γ f f' /\
+             erases Σ Γ L L'.
+Proof.
+  intros. generalize_eqs H.
+  revert f L X.
+  inversion H; intros; try congruence; subst.
+  - inv H4. right. repeat eexists; eauto.
+  - left. split; eauto. econstructor; eauto.
+Qed.
+
+Lemma erases_mkApps Σ Γ f f' L L' :
+  erases Σ Γ f f' ->
+  Forall2 (erases Σ Γ) L L' ->
+  erases Σ Γ (mkApps f L) (E.mkApps f' L').
+Proof.
+  intros. revert f f' H; induction H0; cbn; intros; eauto.
+  eapply IHForall2. econstructor. eauto. eauto.
+Qed.
+
+Lemma erases_mkApps_inv Σ Γ f L T t :
+  wf Σ ->
+  Σ ;;; Γ |- mkApps f L : T ->
+  Σ;;; Γ |- mkApps f L ⇝ℇ t ->
+  (exists L1 L2 L2', L = (L1 ++ L2)%list /\
+                squash (Is_Type_or_Proof Σ Γ (mkApps f L1)) /\
+                erases Σ Γ (mkApps f L1) tBox /\
+                Forall2 (erases Σ Γ) L2 L2' /\
+                t = E.mkApps tBox L2'
+  )
+  \/ exists f' L', t = E.mkApps f' L' /\
+             erases Σ Γ f f' /\
+             Forall2 (erases Σ Γ) L L'.
+Proof.
+  intros wfΣ. intros. revert f X H ; induction L; cbn in *; intros.
+  - right. exists t, []. cbn. repeat split; eauto.
+  - eapply IHL in H; eauto.
+    destruct H as [ (? & ? & ? & ? & [] & ? & ? & ?) | (? & ? & ? & ? & ?)].
+    + subst. left. exists (a :: x), x0, x1. repeat split; eauto.
+    + subst. eapply type_mkApps_inv in X as (? & ? & [] & ?); eauto.
+      eapply erases_App in H0 as [ (-> & []) | (? & ? & ? & ? & ?)].
+      * left. exists [a], L, x0. cbn. repeat split. eauto.
+        econstructor; eauto.  eauto.
+      * subst. right. exists x3, (x4 :: x0). repeat split.
+        eauto. econstructor. eauto. eauto.
+      * eauto.
+Qed.      
+
+(** ** Global erasure  *)
+
+Lemma lookup_env_erases Σ c decl Σ' :
+  wf Σ ->
+  erases_global Σ Σ' ->
+  PCUICTyping.lookup_env (fst Σ) c = Some (ConstantDecl c decl) ->
+  exists decl', ETyping.lookup_env Σ' c = Some (E.ConstantDecl c decl') /\
+           erases_constant_body Σ decl decl'.
+Proof.
+  unfold erases_global. destruct Σ as (Σ, univs).
+  intros. induction H; cbn in *.
+  - inv H0.
+  - destruct ?.
+    + inv H0.
+      exists cb'. split; eauto. unfold erases_constant_body in *.
+      destruct ?. destruct ?. 
+      * eapply erases_extends. 6: eassumption.
+        eapply PCUICWeakeningEnv.wf_extends.
+        eassumption. now eexists [_]. eauto.
+        { inv X. cbn in X1. unfold on_constant_decl in X1. rewrite E0 in *. cbn in X1. eassumption. }
+        eauto. now eexists [_].
+      * eassumption.
+      * destruct ?; tauto.
+    + edestruct IHerases_global_decls as (decl' & ? & ?).
+      eapply PCUICWeakeningEnv.wf_extends.
+      eassumption. now eexists [_]. eauto.
+      exists decl'. split. eauto.
+      unfold erases_constant_body in *. clear H. destruct ?. destruct ?.
+      * eapply erases_extends. 6: eassumption.
+        eapply PCUICWeakeningEnv.wf_extends.
+        eassumption. now eexists [_]. eauto.
+        eapply (PCUICWeakeningEnv.declared_constant_inv (Σ, univs)) in H0; eauto.
+        unfold on_constant_decl in H0. rewrite E0 in H0. unfold lift_typing in H0. eassumption.
+        eapply PCUICWeakeningEnv.weaken_env_prop_typing. eapply PCUICWeakeningEnv.wf_extends. eauto.
+        eexists [_]. reflexivity. eapply PCUICWeakeningEnv.wf_extends. eauto. now eexists [_].
+        eauto. now eexists [_].
+      * tauto.
+      * destruct ?; tauto.
+  - destruct ?.
+    + inv H0.
+    + edestruct IHerases_global_decls as (decl' & ? & ?).
+      eapply PCUICWeakeningEnv.wf_extends.
+      eassumption. now eexists [_]. eauto.
+      exists decl'. split. eauto.
+      unfold erases_constant_body in *. clear H. destruct ?. destruct ?.
+      * eapply erases_extends. 6: eassumption.
+        eapply PCUICWeakeningEnv.wf_extends.
+        eassumption. now eexists [_]. eauto.
+        eapply (PCUICWeakeningEnv.declared_constant_inv (Σ, univs)) in H0; eauto.
+        unfold on_constant_decl in H0. rewrite E0 in H0. unfold lift_typing in H0. eassumption.
+        eapply PCUICWeakeningEnv.weaken_env_prop_typing. eapply PCUICWeakeningEnv.wf_extends. eauto.
+        eexists [_]. reflexivity. eapply PCUICWeakeningEnv.wf_extends. eauto. now eexists [_].
+        eauto. now eexists [_].
+      * tauto.
+      * destruct ?; tauto.
+Qed.        
+
+(** ** The correctness proof  *)
+
+Record extraction_pre (Σ : global_context) : Type
+  := Build_extraction_pre
+  { extr_env_axiom_free' : is_true (axiom_free (fst Σ));
+    extr_env_wf' : wf Σ }.
+
+Hint Constructors PCUICWcbvEval.eval erases.
+
+Lemma erases_correct Σ t T t' v Σ' :
+  extraction_pre Σ ->
+  Σ;;; [] |- t : T ->
+  Σ;;; [] |- t ⇝ℇ t' ->
+   erases_global Σ Σ' ->
+  Σ;;; [] |- t ▷ v ->
+  exists v', Σ;;; [] |- v ⇝ℇ v' /\ Σ' ⊢ t' ▷ v'.
+Proof.
+  intros pre Hty He Heg H.
+  revert T Hty t' He.
+  induction H using PCUICWcbvEval.eval_evals_ind; intros T Hty t' He; inv pre.
+  - assert (Hty' := Hty).
+    assert (eval Σ [] (PCUICAst.tApp f a) res) by eauto.
+    eapply inversion_App in Hty as (? & ? & ? & ? & ? & ?).
+        
+    inv He.
+    + eapply IHeval1 in H4 as (vf' & Hvf' & He_vf'); eauto.
+      eapply IHeval2 in H6 as (vu' & Hvu' & He_vu'); eauto.
+      pose proof (subject_reduction_eval Σ [] _ _ _ extr_env_wf'0 t0 H).
+        eapply inversion_Lambda in X0 as (? & ? & ? & ? & ?).
+        assert (Σ ;;; [] |- a' : t). {
+          eapply subject_reduction_eval; eauto.
+          eapply cumul_Prod_inv in c0 as [].
+          econstructor. eassumption. eauto. eapply c0. }
+      inv Hvf'.
+      * assert (Σ;;; [] |- PCUICLiftSubst.subst1 a' 0 b ⇝ℇ subst1 vu' 0 t').
+        eapply (erases_subst Σ [] [PCUICAst.vass na t] [] b [a'] t'); eauto.
+        econstructor. econstructor. rewrite parsubst_empty. eassumption.
+        eapply IHeval3 in H2 as (v' & Hv' & He_v').
+        -- exists v'. split; eauto.
+           econstructor; eauto.
+        -- eapply substitution0; eauto. 
+      * exists tBox. split. econstructor.
+        eapply Is_type_lambda in X1; eauto.
+        eapply (is_type_subst Σ [] [PCUICAst.vass na _] [] _ [a']) in X1.
+        cbn in X1.
+        eapply Is_type_eval.
+        eauto. eapply H1. eassumption.
+        all: eauto. econstructor. econstructor. rewrite parsubst_empty.
+        eauto. econstructor. eauto.
+    + exists tBox. split. 2:econstructor; eauto.
+      econstructor.
+      eapply Is_type_eval; eauto.
+  - assert (Hty' := Hty).
+    assert (Σ ;;; [] |- tLetIn na b0 t b1 ▷ res) by eauto.
+    eapply inversion_LetIn in Hty' as (? & ? & ? & ? & ? & ?).
+
+    inv He.
+    + eapply IHeval1 in H6 as (vt1' & Hvt2' & He_vt1'); eauto.
+      assert (Hc :red_context Σ ([],, vdef na b0 t) [vdef na b0' t]). {
+        econstructor. econstructor. econstructor. eapply subject_reduction_eval; eauto.
+        eapply wcbeval_red; eauto.         
+      }
+      assert (Σ;;; [vdef na b0' t] |- b1 : x0). {
+        cbn in *. eapply red_context_conversion. 3:eauto. all:eauto. 
+      }
+      assert (Σ;;; [] |- PCUICLiftSubst.subst1 b0' 0 b1 ⇝ℇ subst1 vt1' 0 t2'). {
+        eapply (erases_subst Σ [] [PCUICAst.vdef na b0' t] [] b1 [b0'] t2'); eauto.
+        enough (subslet Σ [] [PCUICLiftSubst.subst [] 0 b0'] [vdef na b0' t]).
+        now rewrite parsubst_empty in X1.
+        econstructor. econstructor.
+        rewrite !parsubst_empty.
+        eapply subject_reduction_eval; eauto.
+        eapply erases_red_context_conversion. 4: eassumption.
+        all: cbn; eauto.
+      }        
+      eapply IHeval2 in H1 as (vres & Hvres & Hty_vres).
+      2:{ eapply substitution_let; eauto. }
+      exists vres. split. eauto. econstructor; eauto.
+    + exists tBox. split. 2:econstructor; eauto.
+      econstructor. eapply Is_type_eval; eauto.
+  - inv isdecl.
+  - inv isdecl.
+  - assert (Hty' := Hty).
+    assert (Σ ;;; [] |- tCase (ind, pars) p discr brs ▷ res) by eauto.
+    eapply inversion_Case in Hty' as (u' & args' & mdecl & idecl & pty & indctx & pctx & ps & btys & ? & ? & ? & ? & ? & ? & ? & ? & ?).
+    assert (Σ ;;; [] |- mkApps (tConstruct ind c u) args :  mkApps (tInd ind u') args').
+    eapply subject_reduction_eval; eauto.
+    eapply type_mkApps_inv in X0 as (? & ? & [] & ?); eauto.
+    eapply inversion_Construct in t1 as (mdecl' & idecl' & cdecl & ? & ? & ? & ?).
+    assert (d1 := d0).
+    destruct d0.
+
+    edestruct (declared_inductive_inj H1 d). subst.
+        
+    pose proof (length_of_btys e0).
+    
+    inv He.
+    + eapply IHeval1 in H11 as (v' & Hv' & He_v'); eauto.
+      eapply erases_mkApps_inv in Hv' as [(? & ? & ? & ? & [] & ? & ? & ?) | (? & ? & ? & ? & ?)]; eauto.
+      3: eapply subject_reduction_eval; eauto.
+      * subst.
+
+        eapply Is_type_app in X0. 2:eauto. 2:{ rewrite mkApps_nested. eapply subject_reduction_eval; eauto. }
+        rewrite mkApps_nested in X0.
+        
+        eapply tConstruct_no_Type in X0.
+        eapply H10 in X0 as []; eauto. 2: exists []; now destruct Σ.
+        
+        destruct (ind_ctors idecl'). cbn in H4. destruct c; inv H2.
+        destruct l; cbn in *; try omega. destruct c as [ | []]; cbn in H2; inv H2.
+
+        destruct btys as [ | ? []]; cbn in H3; try omega. clear H3 H4. destruct H7.
+        (* eapply H7 in d1. *) inv a. inv X2. inv H12. inv H8. destruct H4. destruct x4, y; cbn in *; subst.
+        destruct X1. subst. destruct p0; cbn in *.
+
+        edestruct (IHeval2) as (? & ? & ?).
+        eapply subject_reduction. eauto. exact Hty.
+        etransitivity.
+        eapply PCUICReduction.red_case. econstructor. eapply wcbeval_red. eauto.
+        eapply PCUICReduction.All2_same. intros. econstructor. econstructor. econstructor.
+        econstructor.
+        
+        unfold iota_red. cbn.
+        eapply erases_mkApps. eauto.
+        instantiate (1 := repeat tBox _).
+        eapply All2_Forall.
+        eapply All2_impl.
+        eapply All2_All_mix_left. eassumption.
+        2:{ intros. destruct X1. assert (y = tBox). exact y0. subst. econstructor.
+            now eapply Is_Type_or_Proof_Proof. }
+
+        eapply All2_right_triv. 2: now rewrite repeat_length.
+
+        now eapply All_repeat.
+          
+        (* destruct x4; cbn in e2; subst. destruct X2. destruct p0; cbn in e2; subst. cbn in *.  destruct y.  *)
+        exists x4. split; eauto. eapply eval_iota_sing.  2:eauto.
+        pose proof (Ee.eval_to_value _ _ _ He_v').
+        eapply value_app_inv in H4. subst. eassumption.
+
+        eapply tCase_length_branch_inv in extr_env_wf'0.
+        2:{ eapply subject_reduction. eauto.
+            exact Hty.
+            eapply PCUICReduction.red_case. econstructor. eapply wcbeval_red. eauto.
+            econstructor. econstructor. econstructor. }
+        2: reflexivity.
+
+        enough (#|skipn (ind_npars mdecl') (x1 ++ x2)| = n) as <- by eauto.
+        rewrite skipn_length. rewrite extr_env_wf'0. omega.
+        rewrite extr_env_wf'0. omega.
+      * subst. unfold iota_red in *.
+        destruct (nth_error brs c) eqn:Hnth.
+        2:{ eapply nth_error_None in Hnth. erewrite All2_length in Hnth. 2:exact a. rewrite H3 in Hnth.
+            eapply nth_error_Some_length in H2. cbn in H2. omega.
+        }
+        rewrite <- nth_default_eq in *. unfold nth_default in *.
+        rewrite Hnth in *.
+
+        destruct (All2_nth_error_Some _ _ H12 Hnth) as (? & ? & ? & ?).
+        destruct (All2_nth_error_Some _ _ a Hnth) as (? & ? & ? & ?).
+        destruct p0, x4. cbn in *. subst.
+        edestruct IHeval2 as (? & ? & ?).
+        eapply subject_reduction. eauto. exact Hty.
+        etransitivity.
+        eapply PCUICReduction.red_case. econstructor. eapply wcbeval_red. eauto.
+        eapply PCUICReduction.All2_same. intros. econstructor.
+        etransitivity. eapply trans_red. econstructor.
+        econstructor. unfold iota_red. rewrite <- nth_default_eq. unfold nth_default.
+        rewrite Hnth. econstructor.
+        
+        eapply erases_mkApps. eauto.
+        eapply Forall2_skipn. eauto.
+        inv H5.
+        -- exists x4. split; eauto.
+           econstructor. eauto. unfold ETyping.iota_red.
+           rewrite <- nth_default_eq. unfold nth_default. rewrite e. cbn. eauto.
+        -- eapply Is_type_app in X0. 2:eauto. 2:{ eapply subject_reduction_eval. 3:eassumption. all: eauto. }
+        
+           eapply tConstruct_no_Type in X0.
+           eapply H10 in X0 as []; eauto. 2: exists []; now destruct Σ.
+        
+           destruct (ind_ctors idecl'). cbn in H4. destruct c; inv H2.
+           destruct l; cbn in *; try omega. destruct c as [ | []]; cbn in H2; inv H2.
+           
+           destruct btys as [ | ? []]; cbn in H3; try omega. clear H3 H4. destruct H8.
+           (* eapply H7 in d1. *) inv a. inv X2. inv H12. inv H9. destruct H4. destruct x1, y; cbn in *; subst.
+           destruct X1. subst. destruct p0; cbn in *. destruct x3. inv e. inv Hnth. cbn in *.
+           
+           edestruct (IHeval2) as (? & ? & ?). 
+           eapply subject_reduction. eauto. exact Hty.
+           etransitivity.
+           eapply PCUICReduction.red_case. econstructor. eapply wcbeval_red. eauto.
+           eapply PCUICReduction.All2_same. intros. econstructor. econstructor. econstructor.
+           econstructor.
+
+           eapply erases_mkApps. eauto.
+           instantiate (1 := repeat tBox _).
+           eapply All2_Forall.
+           eapply All2_impl.
+           eapply All2_All_mix_left. eassumption.
+           2:{ intros. destruct X1. assert (y = tBox). exact y0. subst. econstructor.
+               now eapply Is_Type_or_Proof_Proof. }
+
+           eapply All2_right_triv. 2:now rewrite repeat_length.
+           now eapply All_repeat.
+
+           exists x1. split; eauto.
+           eapply eval_iota_sing.
+           pose proof (Ee.eval_to_value _ _ _ He_v').
+           eapply value_app_inv in H4. subst. eassumption. 
+           reflexivity. cbn in *.
+           enough (#|skipn (ind_npars mdecl') args| = n0) as <- by eauto.
+
+           eapply tCase_length_branch_inv in extr_env_wf'0.
+           2:{ eapply subject_reduction. eauto.
+               exact Hty.
+               eapply PCUICReduction.red_case. econstructor. eapply wcbeval_red. eauto.
+               econstructor. econstructor. econstructor. }
+           2: reflexivity.
+
+           enough (#|skipn (ind_npars mdecl') args| = n0) as <- by eauto.
+           rewrite skipn_length. rewrite extr_env_wf'0. omega.
+           rewrite extr_env_wf'0. omega.
+    + exists tBox. split. econstructor. 
+      eapply Is_type_eval; eauto. econstructor; eauto.
+  - assert (Hty' := Hty). 
+    assert (Σ ;;; [] |- mkApps (tFix mfix idx) args ▷ res) by eauto.
+    eapply type_mkApps_inv in Hty' as (? & ? & [] & ?); eauto.
+    eapply EInversion.type_tFix_inv in t as (? & [[] ?] & ?); eauto.
+    unfold unfold_fix in H. rewrite e in H. inv H. 
+
+    eapply erases_mkApps_inv in He as [(? & ? & ? & ? & [] & ? & ? & ?) | (? & ? & ? & ? & ?)]; eauto.
+    + subst.
+      exists tBox. split. 2:eapply eval_box_apps; econstructor; eauto.
+      econstructor. 
+      eapply Is_type_eval. eauto. eassumption.
+      rewrite <- mkApps_nested.
+      eapply Is_type_app. eassumption.
+      rewrite mkApps_nested; eauto.
+      eauto.
+    + subst.
+      inv H3.
+      * assert (Hmfix' := H7).
+        eapply All2_nth_error_Some in H7 as (? & ? & ? & ? & ?); eauto.
+        destruct x1. cbn in *. subst.
+        eapply (erases_subst Σ [] (PCUICLiftSubst.fix_context mfix) [] dbody (fix_subst mfix)) in e3; cbn; eauto.
+        -- enough (exists L, Forall2 (erases Σ []) args' L /\ Forall2 (Ee.eval Σ') x3 L). 
+           ++ cbn in e3. destruct H as (L & ? & ?).
+              assert (Hv : Forall Ee.value L).
+              { eapply Forall2_Forall_right; eauto.
+                intros. eapply EWcbvEval.eval_to_value. eauto.
+              } 
+                
+              eapply erases_mkApps in e3; eauto.
+              eapply IHeval in e3 as (? & ? & ?); cbn; eauto.
+              exists x1. split. eauto. econstructor. unfold ETyping.unfold_fix.
+              rewrite e0. reflexivity.
+              eassumption.
+              all:eauto.
+              ** unfold is_constructor in *.
+                 destruct ?; inv H1.
+                 unfold is_constructor_or_box.
+                 eapply Forall2_nth_error_Some in H as (? & ? & ?); eauto.
+                 rewrite H.
+                 
+                 unfold isConstruct_app in H8.
+                 destruct (decompose_app t) eqn:EE.
+                 assert (E2 : fst (decompose_app t) = t1) by now rewrite EE. 
+                 destruct t1.
+                 all:inv H8.
+                 (* erewrite <- PCUICConfluence.fst_decompose_app_rec in E2. *)
+                 
+                 pose proof (PCUICConfluence.decompose_app_rec_inv EE).
+                 cbn in H7. subst.
+                 assert (∑ T, Σ ;;; [] |- mkApps (tConstruct ind n ui) l : T) as [T' HT'].
+                 { eapply typing_spine_eval in t0; eauto.
+                   eapply typing_spine_In; eauto.
+                   eapply nth_error_In; eauto. }
+                 eapply erases_mkApps_inv in H1.
+                 destruct H1 as [ (? & ? & ? & ? & [] & ? & ? & ?) | (? & ? & ? & ? & ?) ].
+                 --- subst.
+                     eapply nth_error_forall in Hv; eauto.
+                     eapply value_app_inv in Hv. subst. reflexivity.
+                 --- subst. inv H7. 
+                     +++ eapply nth_error_forall in Hv; eauto.
+                         destruct x6 using rev_ind; cbn - [EAstUtils.decompose_app]. reflexivity.
+                         rewrite emkApps_snoc at 1.
+                         generalize (x6 ++ [x4])%list. clear. intros.
+                         rewrite Prelim.decompose_app_mkApps. reflexivity.
+                         reflexivity.
+                     +++ eapply nth_error_forall in Hv; eauto.
+                         eapply value_app_inv in Hv. subst. eauto.                         
+                 --- eauto.
+                 --- eauto.
+              ** eapply type_mkApps.
+                 --- eapply (substitution Σ [] (PCUICLiftSubst.fix_context mfix) (fix_subst mfix) []); eauto.
+                     
+                     eapply subslet_fix_subst.
+                     eapply nth_error_all in a0; eauto. cbn in a0.
+                     eapply a0.
+                 --- cbn.
+                     eapply typing_spine_eval in t0. 2-5:eauto.
+                     rewrite (plus_n_O #|PCUICLiftSubst.fix_context mfix|).
+                     rewrite fix_context_length.
+                     rewrite <- fix_subst_length.
+                     rewrite PCUICLiftSubst.simpl_subst.
+                     now rewrite PCUICLiftSubst.lift0_id. omega.
+           ++ clear - t0 H0 H4. revert x t0 x3 H4; induction H0; intros.
+              ** inv H4. exists []; eauto.
+              ** inv H4. inv t0. eapply r in H2 as (? & ? & ?); eauto.
+                 eapply IHAll2 in H5 as (? & ? & ?); eauto.
+        -- eapply subslet_fix_subst.
+        -- eapply nth_error_all in a0; eauto. cbn in a0.
+           eapply a0.
+        -- eapply All2_from_nth_error.
+           erewrite fix_subst_length, ETyping.fix_subst_length, All2_length; eauto.
+           intros.
+           rewrite fix_subst_nth in H3. 2:{ now rewrite fix_subst_length in H. }
+           rewrite efix_subst_nth in H5. 2:{ rewrite fix_subst_length in H.
+                                             erewrite <- All2_length; eauto. }
+           inv H3; inv H5.
+           erewrite All2_length; eauto.
+      * exists tBox. split.
+        econstructor. 
+        eapply Is_type_eval. eauto. eassumption.
+        eapply Is_type_app. eauto. eauto. eauto.
+        eapply eval_box_apps. econstructor. eauto.
+  - destruct Σ as (Σ, univs).
+    unfold erases_global in Heg.
+    assert (Σ ;;; [] |- tConst c u ▷ res) by eauto.
+    (* eapply type_Const_inv in Hty. *)    
+    inv He.
+    + assert (H' := H).
+      eapply lookup_env_erases in H; eauto.
+      destruct H as (decl' & ? & ?).
+      unfold erases_constant_body in H2. rewrite H0 in *.
+      destruct ?; try tauto.
+      edestruct IHeval.
+      * eapply typing_subst_instance. eauto.
+        eapply PCUICWeakeningEnv.declared_constant_inv in H'; eauto.
+        unfold on_constant_decl in H'. rewrite H0 in H'. eapply H'.
+        eapply PCUICWeakeningEnv.weaken_env_prop_typing.
+      * eapply erases_subst_instance_constr; eauto.
+        eapply PCUICWeakeningEnv.declared_constant_inv in H'; eauto.
+        unfold on_constant_decl in H'. rewrite H0 in H'. eapply H'.
+        eapply PCUICWeakeningEnv.weaken_env_prop_typing.        
+      * destruct H3. exists x. split; eauto. econstructor; eauto.
+    + exists tBox. split. econstructor.
+      eapply Is_type_eval. 3: eassumption. eauto. eauto. econstructor. eauto.
+  - pose (Hty' := Hty).
+    eapply inversion_Proj in Hty' as (? & ? & ? & [] & ? & ? & ? & ? & ?). 
+    inv He.
+    + rename H7 into H6. eapply IHeval1 in H6 as (vc' & Hvc' & Hty_vc'); eauto.
+      eapply erases_mkApps_inv in Hvc'; eauto.
+      2: eapply subject_reduction_eval; eauto.
+      destruct Hvc' as [ (? & ? & ? & ? & [] & ? & ? & ?) | (? & ? & ? & ? & ?)]; subst.
+      * exists tBox. split.
+
+        eapply Is_type_app in X; eauto. 2:{ rewrite mkApps_nested. eapply subject_reduction_eval; eauto. }
+        rewrite mkApps_nested in X.
+        
+        eapply tConstruct_no_Type in X. eapply H5 in X as [? []]; eauto.
+        2: now destruct d. 2: now exists []; destruct Σ.
+                                    
+        econstructor. 
+        eapply Is_type_eval. eauto. eauto.
+        eapply nth_error_all.
+        eapply nth_error_skipn. eassumption.
+        eapply All_impl. assert (pars = ind_npars x0). destruct d as (? & ? & ?). now rewrite H9. subst.
+        eassumption.
+        eapply Is_Type_or_Proof_Proof.
+
+        eapply eval_proj_box.
+        pose proof (Ee.eval_to_value _ _ _ Hty_vc').
+        eapply value_app_inv in H3. subst. eassumption.        
+      * rename H5 into Hinf.
+        rename H6 into H5.
+        eapply Forall2_nth_error_Some in H5 as (? & ? & ?); eauto.
+        assert (Σ ;;; [] |- mkApps (tConstruct i k u) args : mkApps (tInd i x) x2).
+        eapply subject_reduction_eval; eauto.
+        eapply type_mkApps_inv in X as (? & ? & [] & ?); eauto.
+        eapply typing_spine_In in t2 as [].
+        2: eapply nth_error_In; eauto.
+        eapply IHeval2 in H5 as (? & ? & ?); eauto. 
+        inv H4.
+        -- exists x9. split; eauto. econstructor. eauto.
+           rewrite <- nth_default_eq. unfold nth_default. now rewrite H3.
+        -- exists tBox. split.
+
+           eapply Is_type_app in X; eauto. 2:{ eapply subject_reduction_eval. 3: eauto. eauto. eauto. }
+           
+           eapply tConstruct_no_Type in X. eapply Hinf in X as [? []]; eauto.
+           2: now destruct d. 2: now exists []; destruct Σ.
+                                       
+           econstructor. 
+           eapply Is_type_eval. eauto. eauto.
+           eapply nth_error_all.
+           eapply nth_error_skipn. eassumption.
+           eapply All_impl. assert (pars = ind_npars x0). destruct d as (? & ? & ?). now rewrite H9. subst.
+           eassumption.
+           eapply Is_Type_or_Proof_Proof.
+
+           eapply eval_proj_box.
+           pose proof (Ee.eval_to_value _ _ _ Hty_vc').
+           eapply value_app_inv in H4. subst. eassumption.
+    + exists tBox. split. econstructor.
+      eapply Is_type_eval. 3: eassumption. eauto. eauto. econstructor. eauto.
+  - inv He.
+    + eexists. split; eauto. econstructor.
+    + eexists. split; eauto. now econstructor.
+  - inv He. eexists. split; eauto. now econstructor.
+  - inv He. eexists. split; eauto. now econstructor.
+  - assert (Σ ;;; [] |- mkApps (tInd i u) l' : T).
+    eapply subject_reduction_eval; eauto; econstructor; eauto.
+    assert (Hty' := X0).
+    eapply type_mkApps_inv in X0 as (? & ? & [] & ?); eauto.
+    assert (Hty'' := Hty).
+    eapply type_mkApps_inv in Hty'' as (? & ? & [] & ?); eauto.
+    Require Import PCUIC.PCUICInversion.
+    eapply inversion_Ind in t as (? & ? & ? & ? & ? & ?).
+    eapply erases_mkApps_inv in Hty; eauto.
+    destruct Hty as [ (? & ? & ? & ? & [] & ? & ? & ?) | (? & ? & ? & ? & ?)].
+    + subst. exists tBox.
+      split. 2:{ eapply eval_box_apps. now econstructor. }
+      econstructor. eauto.
+      eapply All2_app_inv in X as ([] & [] & ?). subst.
+      rewrite <- mkApps_nested. 
+      eapply Is_type_app. eauto.
+      rewrite mkApps_nested. eauto.
+      eapply Is_type_eval. eauto.
+      eapply eval_app_ind. eauto. eauto.
+      eauto.
+    + subst. exists tBox.
+      eapply IHeval in H2 as (? & ? & ?).
+      inv H1.
+      split. econstructor.
+      eauto. eapply Is_type_app; eauto.
+      eapply eval_box_apps; eauto. eauto.
+  - inv He.
+    + eexists. split; eauto. now econstructor.
+    + eexists. split. 2: now econstructor.
+      econstructor; eauto.
+  - assert (Hty' := Hty).
+    assert (Hty'' : Σ ;;; [] |- mkApps (tConstruct i k u) l' : T). {
+      eapply subject_reduction. eauto. eapply Hty.
+      eapply PCUICReduction.red_mkApps.
+      eapply wcbeval_red; eauto.
+      eapply All2_impl. exact X. intros.
+      eapply wcbeval_red; eauto.
+    }
+    eapply erases_mkApps_inv in Hty; eauto.
+    destruct Hty as [ (? & ? & ? & ? & [] & ? & ? & ?) | (? & ? & ? & ? & ?)].
+    + subst. exists tBox.
+      split. 2:{ eapply eval_box_apps. now econstructor. }
+      eapply All2_app_inv in X as ( [] & [] & ?). subst.
+      econstructor.
+
+      rewrite <- mkApps_nested. 
+      eapply Is_type_app. eauto.
+      rewrite mkApps_nested. eauto.
+      eapply Is_type_red. eauto.
+      eapply PCUICReduction.red_mkApps.
+      eapply wcbeval_red; eauto.
+      eapply All2_impl. exact a. intros.
+      eapply wcbeval_red; eauto. eauto. 
+    + subst.
+      eapply type_mkApps_inv in Hty' as (? & ? & [] & ?); eauto.
+      eapply IHeval in H2 as (? & ? & ?); eauto.
+      enough (exists l'', Forall2 (erases Σ []) l' l'' /\ Forall2 (Ee.eval Σ') x0 l'').
+      * destruct H4 as [l''].
+        inv H1.
+        -- exists (E.mkApps (E.tConstruct i k) l''). split.
+           eapply erases_mkApps; eauto.
+           firstorder. econstructor; firstorder.
+        -- exists tBox.
+           split.
+           econstructor. eauto. eapply Is_type_app; eauto.
+           eapply eval_box_apps. eauto.
+      * clear - t0 H0 H3. revert x1 x0 H3 t0. induction H0; intros.
+        -- inv H3. eauto.
+        -- inv H3. inv t0. eapply IHAll2 in H5 as (? & ? & ?).
+           eapply r in H2 as (? & ? & ?); eauto. 
+           eauto.
+Qed.
