extraction/theories/Prelim.v
@@ -1,0 +1,231 @@
+(* Distributed under the terms of the MIT license.   *)
+
+From Coq Require Import Bool String List Program BinPos Compare_dec Omega Lia.
+From MetaCoq.Template Require Import config utils monad_utils BasicAst AstUtils.
+From MetaCoq.PCUIC Require Import PCUICAst PCUICAstUtils PCUICInduction PCUICTyping PCUICWeakening PCUICSubstitution PCUICSafeChecker PCUICRetyping PCUICMetaTheory PCUICWcbvEval PCUICSR  PCUICClosed PCUICGeneration.
+From MetaCoq.Extraction Require Import EAst ELiftSubst ETyping EWcbvEval Extract.
+From Equations Require Import Equations.
+Require Import String.
+Local Open Scope list_scope.
+Set Asymmetric Patterns.
+Import MonadNotation.
+
+
+Existing Instance config.default_checker_flags.
+Module PA := PCUICAst.
+Module P := PCUICWcbvEval.
+
+Lemma nth_error_app_inv X (x : X) n l1 l2 :
+  nth_error (l1 ++ l2) n = Some x -> (n < #|l1| /\ nth_error l1 n = Some x) \/ (n >= #|l1| /\ nth_error l2 (n - List.length l1) = Some x).
+Proof.
+  destruct (le_lt_dec #|l1| n).
+  - intros. rewrite nth_error_app2 in H; eauto.
+  - intros. rewrite nth_error_app1 in H; eauto.
+Qed.
+
+
+Lemma monad_map_All2 (X Y : Type) (f : X -> typing_result Y) (l1 : list X) (a1 : list Y) :
+  monad_map f l1 = ret a1 -> All2 (fun a b => f a = ret b) l1 a1.
+Proof.
+  induction l1 in a1 |- *; cbn; intros.
+  - inv H. econstructor.
+  - repeat destruct ? in H; try congruence.
+    inv H. econstructor; eauto.
+Qed.
+    
+Lemma monad_map_Forall2 (X Y : Type) (f : X -> typing_result Y) (l1 : list X) (a1 : list Y) :
+  monad_map f l1 = Checked a1 -> Forall2 (fun a b => f a = Checked b) l1 a1.
+Proof.
+  intros. now eapply All2_Forall, monad_map_All2.
+Qed.
+  
+Lemma monad_map_length X Y (f : X -> typing_result Y) (l1  : list X) a :
+  monad_map f l1 = Checked a -> #|l1| = #|a|.
+Proof.
+  revert a; induction l1; cbn; intros.
+  - invs H. cbn. congruence.
+  - destruct (f a). destruct ? in H. invs H. cbn. f_equal. eauto. invs H. invs H.
+Qed.
+
+
+Lemma monad_map_app X Y (f : X -> typing_result Y) (l1 l2 : list X) a1 a2 :
+  monad_map f l1 = Checked a1 -> monad_map f l2 = Checked a2 -> monad_map f (l1 ++ l2) = Checked (a1 ++ a2)%list.
+Proof.
+  revert a1. induction l1; intros.
+  - cbn in *. invs H. eauto.
+  - cbn in *. destruct ?. destruct ? in H; try congruence.
+    invs H. rewrite (IHl1 _ eq_refl); eauto. invs H.
+Qed.
+
+Lemma monad_map_app_invs X Y (f : X -> typing_result Y) (l1 l2 : list X) a :
+  monad_map f (l1 ++ l2) = Checked a -> exists a1 a2, monad_map f l1 = Checked a1 /\ monad_map f l2 = Checked a2 /\ (a = a1 ++ a2)%list.
+Proof.
+  intros. revert a H. induction l1; intros.
+  - cbn in *. eauto.
+  - cbn in *. destruct ?. destruct ? in H; try congruence.
+    invs H. destruct (IHl1 _ eq_refl) as (? & ? & ? & ? & ->).
+    do 2 eexists. rewrite H. eauto. invs H.
+Qed.
+
+Lemma typing_spine_inv_app Σ x0 l x x1 :
+  PCUICGeneration.typing_spine Σ [] x0 (l ++ [x]) x1 -> { '(x2, x3) : _ & (PCUICGeneration.typing_spine Σ [] x0 l x2) * (Σ ;;; [] |- x : x3)}%type.
+Proof.
+  intros. depind X. destruct l; inv H.
+  destruct l; invs H.
+  + eexists (_, _). split. econstructor. eauto.
+  + specialize (IHX _ _ _ _ eq_refl) as ([] & []).
+    eexists (_, _). split.  econstructor; eauto. eauto.
+Qed.
+
+Lemma typing_spine_inv:
+  forall (Σ : PCUICAst.global_context) (i : inductive) (pars arg : nat) (args : list PCUICAst.term) 
+    (a T : PCUICAst.term) (args' : list PCUICAst.term) (u' : universe_instance)
+    (H17 : nth_error args (pars + arg) = Some a) (x2 x3 : PCUICAst.term),
+    PCUICGeneration.typing_spine Σ [] x2 args x3 ->
+    Σ;;; [] |- x3 <= PCUICAst.mkApps (tInd (fst (fst (i, pars, arg))) u') args' -> {T & Σ;;; [] |- a : T}.
+Proof.
+  intros. simpl in *.
+  revert pars arg H17.
+  dependent induction X; intros pars arg H17.
+  - rewrite nth_error_nil in H17. congruence.
+  - destruct (pars + arg)%nat eqn:E.
+    + cbn in H17. invs H17. eauto.
+    + cbn in H17. eapply IHX.
+      eauto. instantiate (2 := 0). eassumption.
+Qed.
+
+Lemma typing_spine_cumul:
+  forall (Σ : PCUICAst.global_context) (T x1 : PCUICAst.term), Σ;;; [] |- x1 <= T -> typing_spine Σ [] x1 [] T.
+Proof.
+  intros Σ T x1 X.
+Admitted.
+
+Theorem subject_reduction_eval : forall (Σ : PCUICAst.global_context) Γ t u T,
+  wf Σ -> Σ ;;; Γ |- t : T -> PCUICWcbvEval.eval Σ Γ t u -> Σ ;;; Γ |- u : T.
+Proof.
+  intros * wfΣ Hty Hred % wcbeval_red. eapply subject_reduction; eauto.
+Qed.
+
+Lemma typing_spine_eval:
+  forall (Σ : PCUICAst.global_context) (args args' : list PCUICAst.term) (X : All2 (PCUICWcbvEval.eval Σ []) args args') (bla : wf Σ)
+    (T x x0 : PCUICAst.term) (t0 : typing_spine Σ [] x args x0) (c : Σ;;; [] |- x0 <= T) (x1 : PCUICAst.term)
+    (c0 : Σ;;; [] |- x1 <= x), typing_spine Σ [] x1 args' T.
+Proof.
+  intros Σ args args' X wf T x x0 t0 c x1 c0. revert args' X.
+  dependent induction t0; intros.
+  - inv X.
+    eapply (typing_spine_cumul). eapply cumul_trans; eauto.
+  - inv X. econstructor.
+    + eauto.
+    + eapply cumul_trans; eauto.
+    + eapply subject_reduction_eval; eauto.
+    + eapply IHt0; eauto.
+      eapply PCUICCumulativity.red_cumul_inv.
+      unfold PCUICLiftSubst.subst1.
+      eapply (red_red Σ [] [_] [] [_] [_]).
+      eauto. econstructor. eapply wcbeval_red. eauto.
+      econstructor. econstructor. econstructor. now rewrite parsubst_empty.
+      Grab Existential Variables. econstructor.
+Qed.
+
+
+(* Lemma typing_spine_skipn: *)
+(*   forall (Σ : PCUICAst.global_context) (args : list PCUICAst.term) (n0 : nat) (t5 x x0 : PCUICAst.term)  *)
+(*     (n : nat) (t3 : PCUICGeneration.typing_spine Σ [] x args x0), *)
+(*     {T & PCUICGeneration.typing_spine Σ [] (snd (n0, t5)) (skipn n args) T}. *)
+(* Proof. *)
+(*   intros Σ args n0 t5 x x0. intros. *)
+(*   revert n. dependent induction t3; intros. *)
+(*   - cbn. destruct n; unfold skipn; repeat econstructor. *)
+(*   - cbn in *. destruct n. *)
+(*     + unfold skipn. econstructor. econstructor; eauto. *)
+(*       destruct (IHt3 0). *)
+(*       assert (skipn 0 tl = tl) by now destruct tl. *)
+(*       admit. *)
+(*     + unfold skipn. fold (skipn n tl). eauto.       *)
+(* Admitted. *)
+
+(** ** on mkApps *)
+
+Lemma emkApps_snoc a l b :
+  mkApps a (l ++ [b]) = tApp (mkApps a l) b.
+Proof.
+  revert a; induction l; cbn; congruence.
+Qed.
+
+Lemma mkApps_snoc a l b :
+  PCUICAst.mkApps a (l ++ [b]) = PCUICAst.tApp (PCUICAst.mkApps a l) b.
+Proof.
+  revert a; induction l; cbn; congruence.
+Qed.
+
+Lemma mkAppBox_repeat n a :
+  mkAppBox a n = mkApps a (repeat tBox n).
+Proof.
+  revert a; induction n; cbn; firstorder congruence.
+Qed.
+
+(* TODO: move *)
+
+(* Lemma is_type_extract (Σ : PCUICAst.global_context) Γ (t : PCUICAst.term) (* T : *) *)
+(*   (* Σ ;;; Γ |- t : T -> *) : *)
+(*   Extract.is_type_or_proof Σ Γ t = true -> extract Σ Γ t = E.tBox. *)
+(* Proof. *)
+(*   (* split. *) *)
+(*   (* - intros H1. *) *)
+(*   (*   destruct t; simpl; try rewrite H1; try reflexivity. *) *)
+(*   (*   all: try inversion H1. *) *)
+(*   (* - intros. *) *)
+(*   (* (* - intros. induction X. *) *) *)
+(*   (* (*   all: simpl in H0; try destruct ?; try destruct a0. all: try congruence. *) *) *)
+(*   (* (*   cbn in E. destruct is_arity eqn:EE. inv E. *) *) *)
+(*   (* (*   all: try now destruct ?; congruence. *) *) *)
+(*   (* (*   cbn in E. destruct H. cbn in E. inv E. *) *) *)
+(* Admitted. *)
+
+(* Theorem type_of_sound `{Fuel} Σ {Γ t A B} : *)
+(*       Σ ;;; Γ |- t : A -> *)
+(*       type_of Σ Γ t = Checked B -> *)
+(*       (Σ ;;; Γ |- t : B) * (Σ ;;; Γ |- B <= A). *)
+(* Admitted. *)
+
+(* Theorem type_of_complete `{Fuel} Σ {Γ t A} : *)
+(*       Σ ;;; Γ |- t : A -> *)
+(*                     {B & type_of Σ Γ t = Checked B}. *)
+(* Admitted. *)
+
+
+Lemma decompose_app_rec_mkApps f l l' : EAstUtils.decompose_app_rec (mkApps f l) l' =
+                                    EAstUtils.decompose_app_rec f (l ++ l').
+Proof.
+  induction l in f, l' |- *; simpl; auto; rewrite IHl, ?app_nil_r; auto.
+Qed.
+
+Lemma decompose_app_mkApps f l :
+  isApp f = false -> EAstUtils.decompose_app (mkApps f l) = (f, l).
+Proof.
+  intros Hf. unfold EAstUtils.decompose_app. rewrite decompose_app_rec_mkApps. rewrite app_nil_r.
+  destruct f; simpl in *; (discriminate || reflexivity).
+Qed.
+
+Lemma typing_spine_In:
+  forall (Σ : PCUICAst.global_context) (args : list PCUICAst.term) 
+    (x x0 : PCUICAst.term) (t0 : typing_spine Σ [] x args x0) 
+    (x1 : PCUICAst.term) (H : In x1 args), ∑ T1, Σ;;; [] |- x1 : T1.
+Proof.
+  intros Σ args x x0 t0 x1 H.
+Admitted.
+
+
+Lemma fix_subst_length mfix :
+  #|PCUICTyping.fix_subst mfix| = #|mfix|.
+Proof.
+Admitted.
+Lemma fix_context_length mfix :
+  #|PCUICLiftSubst.fix_context mfix| = #|mfix|.
+Proof.
+Admitted.
+Lemma fix_subst_length' mfix :
+  #|fix_subst mfix| = #|mfix|.
+Proof.
+Admitted.
